jar2bpl_test/regression/false_positives/fp10/FalsePositive10.java
@@ -2,6 +2,8 @@
 
 public class FalsePositive10 {
 
+	//two snippets from terpword that were reported but are false positives.
+	
 	public void foo(char[] temp) {
 		int end = -1;
 		int j = temp.length;
@@ -13,4 +15,38 @@ public class FalsePositive10 {
 		} while (end == -1 && j >= 0);
 		j = end;		
 	}
+	
+	private String getText() {return "";}
+	
+	/**
+	 * @return boolean - true if image is valid
+	 */
+	public boolean validateControls()
+	{
+		boolean result = true;
+		if(!getText().equals(""))
+		{
+			try
+			{
+				Integer.parseInt(getText());
+			}
+			catch (NumberFormatException e)
+			{
+				result = false;
+			}
+		}
+		if( result && !getText().equals(""))
+		{
+			try
+			{
+				Integer.parseInt(getText());
+			}
+			catch (NumberFormatException e)
+			{
+				result = false;
+			}
+		}
+		return result;
+	}	
+	
 }
