jar2bpl_test/regression/true_positives/tp04/TruePositive04.java
@@ -1,0 +1,50 @@
+
+
+import java.awt.BorderLayout;
+import java.awt.Color;
+import java.awt.Container;
+import java.awt.Dimension;
+import java.awt.Font;
+import java.awt.GridLayout;
+import java.awt.Insets;
+import java.awt.font.FontRenderContext;
+import java.awt.geom.Rectangle2D;
+
+import javax.swing.ButtonGroup;
+import javax.swing.JButton;
+import javax.swing.JComboBox;
+import javax.swing.JLabel;
+import javax.swing.JPanel;
+import javax.swing.JToggleButton;
+import javax.swing.SwingConstants;
+import javax.swing.WindowConstants;
+
+public class TruePositive04 {
+	
+	private static final int UNICODEBLOCKSIZE = 0;
+	private Object parentEkit;
+	private Font buttonFont;
+	private JToggleButton[] buttonArray = new JToggleButton[UNICODEBLOCKSIZE];
+	private ButtonGroup buttonGroup;
+	private JComboBox jcmbBlockSelector;
+	private JComboBox jcmbPageSelector;
+	
+	/**
+	 * creates and initializes the unicode dialog 
+	 * @param startIndex - index of selected text
+	 */
+	public void init(int startIndex)
+	{
+		String customFont = "";
+		if(customFont != null && customFont.length() > 0)
+		{
+			buttonFont = new Font("", Font.PLAIN, 12);
+		}
+		else
+		{
+			buttonFont = new Font("Monospaced", Font.PLAIN, 12); //that should be unreachable
+		}
+	}
+
+
+}
