jar2bpl_test/test_tmp_boogiefiles/fp01.bpl
@@ -16,8 +16,11 @@ const unique $StringConst0 : ref extends  complete;
 const { :sourceloc "/Users/schaef/git/jar2bpl/jar2bpl_test/regression/false_positives/fp01/FalsePositives01.java",-1,-1,-1,-1 } unique java.io.Serializable : javaType extends  unique java.lang.Object complete;
 const { :sourceloc "/Users/schaef/git/jar2bpl/jar2bpl_test/regression/false_positives/fp01/FalsePositives01.java",-1,-1,-1,-1 } unique java.lang.Comparable : javaType extends  unique java.lang.Object complete;
 const { :sourceloc "/Users/schaef/git/jar2bpl/jar2bpl_test/regression/false_positives/fp01/FalsePositives01.java",-1,-1,-1,-1 } unique java.lang.CharSequence : javaType extends  unique java.lang.Object complete;
-const { :sourceloc "/Users/schaef/git/jar2bpl/jar2bpl_test/regression/false_positives/fp01/FalsePositives01.java",-1,-1,-1,-1 } unique java.lang.String : javaType extends  unique java.io.Serializable, unique java.lang.Object, unique java.lang.CharSequence, unique java.lang.Comparable complete;
+const { :sourceloc "/Users/schaef/git/jar2bpl/jar2bpl_test/regression/false_positives/fp01/FalsePositives01.java",-1,-1,-1,-1 } unique java.lang.String : javaType extends  unique java.lang.CharSequence, unique java.io.Serializable, unique java.lang.Comparable, unique java.lang.Object complete;
 const { :sourceloc "/Users/schaef/git/jar2bpl/jar2bpl_test/regression/false_positives/fp01/FalsePositives01.java",-1,-1,-1,-1 } unique java.lang.Throwable : javaType extends  unique java.io.Serializable, unique java.lang.Object complete;
+const { :sourceloc "/Users/schaef/git/jar2bpl/jar2bpl_test/regression/false_positives/fp01/FalsePositives01.java",-1,-1,-1,-1 } unique java.lang.Exception : javaType extends  unique java.lang.Throwable complete;
+const { :sourceloc "/Users/schaef/git/jar2bpl/jar2bpl_test/regression/false_positives/fp01/FalsePositives01.java",-1,-1,-1,-1 } unique java.lang.RuntimeException : javaType extends  unique java.lang.Exception complete;
+const { :sourceloc "/Users/schaef/git/jar2bpl/jar2bpl_test/regression/false_positives/fp01/FalsePositives01.java",-1,-1,-1,-1 } unique java.lang.ClassCastException : javaType extends  unique java.lang.RuntimeException complete;
 const unique $StringConst1 : ref extends  complete;
 const unique $StringConst2 : ref extends  complete;
 const unique $StringConst3 : ref extends  complete;
@@ -52,9 +55,9 @@ function $shlInt(x:int, y:int) returns ($ret:int);
 function $ushrInt(x:int, y:int) returns ($ret:int);
 function $shrInt(x:int, y:int) returns ($ret:int);
 axiom (forall t : javaType :: $heap[$null,$type] <: t);
-procedure $new(obj_type:javaType) returns ($obj:ref);    ensures $heap[$obj,$alloc] == true;    requires $heap[$obj,$alloc] == false;        ensures $heap[$obj,$type] == obj_type;    ensures $obj != $null;
+procedure $new(obj_type:javaType) returns ($obj:ref);        ensures $heap[$obj,$alloc] == true;    ensures $heap[$obj,$type] == obj_type;    requires $heap[$obj,$alloc] == false;    ensures $obj != $null;
 
-procedure java.lang.Object$java.lang.Object$clone$43($this:ref) returns ($other:ref);    ensures $heap[$other,$alloc] == true;        ensures $heap[$other,$type] == $heap[$this,$type];    ensures $other != $null;
+procedure java.lang.Object$java.lang.Object$clone$43($this:ref) returns ($other:ref);        ensures $heap[$other,$alloc] == true;    ensures $other != $null;    ensures $heap[$other,$type] == $heap[$this,$type];
 
 procedure int$java.lang.String$compareTo$87($this:ref, $other:ref) returns ($return:int);    
 
@@ -82,8 +85,8 @@ procedure void$java.lang.Object$$la$init$ra$$38($this:ref) returns ($exception:r
 
 implementation int$FalsePositives01$foo$1889($this:ref) returns ($return:int, $exception:ref){
     
-var this1 : ref;    
-var temp$02 : int;
+var temp$02 : int;    
+var this1 : ref;
     assume { :sourceloc "/Users/schaef/git/jar2bpl/jar2bpl_test/regression/false_positives/fp01/FalsePositives01.java",-1,-1,-1,-1 } $this != $null;
     assert { :sourceloc "/Users/schaef/git/jar2bpl/jar2bpl_test/regression/false_positives/fp01/FalsePositives01.java",23,2,23,29 } true;
     this1 := $this;
@@ -97,8 +100,8 @@ var temp$02 : int;
 
 implementation java.util.Enumeration$FalsePositives01$bar$1890($this:ref) returns ($return:ref, $exception:ref){
     
-var temp$04 : ref;    
-var this3 : ref;
+var this3 : ref;    
+var temp$04 : ref;
     assume { :sourceloc "/Users/schaef/git/jar2bpl/jar2bpl_test/regression/false_positives/fp01/FalsePositives01.java",-1,-1,-1,-1 } $this != $null;
     assume $heap[$return,$type] <: java.util.Enumeration;
     assert { :sourceloc "/Users/schaef/git/jar2bpl/jar2bpl_test/regression/false_positives/fp01/FalsePositives01.java",24,2,24,40 } true;
@@ -113,23 +116,23 @@ var this3 : ref;
 
 implementation void$FalsePositives01$removeAttribute$1891($this:ref) returns ($exception:ref){
     
-var temp$311 : ref;    
-var temp$1220 : int;    
-var hit6 : int;    
-var temp$816 : int;    
-var temp$19 : int;    
-var temp$513 : ref;    
-var temp$1018 : ref;    
-var countSource7 : int;    
-var temp$412 : int;    
-var temp$917 : ref;    
-var temp$614 : int;    
-var cce21 : ref;    
-var temp$715 : ref;    
 var temp$1119 : int;    
-var this5 : ref;    
+var temp$816 : int;    
+var temp$311 : ref;    
+var temp$917 : ref;    
 var temp$210 : int;    
-var temp$08 : ref;
+var temp$08 : ref;    
+var cce21 : ref;    
+var temp$19 : int;    
+var hit6 : int;    
+var temp$1220 : int;    
+var temp$1018 : ref;    
+var temp$513 : ref;    
+var temp$412 : int;    
+var temp$715 : ref;    
+var countSource7 : int;    
+var this5 : ref;    
+var temp$614 : int;
     assume { :sourceloc "/Users/schaef/git/jar2bpl/jar2bpl_test/regression/false_positives/fp01/FalsePositives01.java",-1,-1,-1,-1 } $this != $null;
     assert { :sourceloc "/Users/schaef/git/jar2bpl/jar2bpl_test/regression/false_positives/fp01/FalsePositives01.java",26,2,52,2 } true;
     this5 := $this;
@@ -150,8 +153,6 @@ var temp$08 : ref;
     if (countSource7 < temp$19) {
         assert { :sourceloc "/Users/schaef/git/jar2bpl/jar2bpl_test/regression/false_positives/fp01/FalsePositives01.java",32,43,32,52 } true;
         goto block3;
-    } else {
-        assert { :sourceloc "/Users/schaef/git/jar2bpl/jar2bpl_test/regression/false_positives/fp01/FalsePositives01.java",32,43,32,52 } true;
     }
     assert { :sourceloc "/Users/schaef/git/jar2bpl/jar2bpl_test/regression/false_positives/fp01/FalsePositives01.java",32,43,32,52 } true;
     goto block4;
@@ -172,8 +173,6 @@ var temp$08 : ref;
     if (temp$513 == $StringConst0) {
         assert { :sourceloc "/Users/schaef/git/jar2bpl/jar2bpl_test/regression/false_positives/fp01/FalsePositives01.java",35,8,35,17 } true;
         goto block5;
-    } else {
-        assert { :sourceloc "/Users/schaef/git/jar2bpl/jar2bpl_test/regression/false_positives/fp01/FalsePositives01.java",35,8,35,17 } true;
     }
     assert { :sourceloc "/Users/schaef/git/jar2bpl/jar2bpl_test/regression/false_positives/fp01/FalsePositives01.java",35,8,35,17 } true;
     goto block6;
@@ -189,8 +188,6 @@ var temp$08 : ref;
     if (hit6 == 0) {
         assert { :sourceloc "/Users/schaef/git/jar2bpl/jar2bpl_test/regression/false_positives/fp01/FalsePositives01.java",41,9,41,11 } true;
         goto block7;
-    } else {
-        assert { :sourceloc "/Users/schaef/git/jar2bpl/jar2bpl_test/regression/false_positives/fp01/FalsePositives01.java",41,9,41,11 } true;
     }
     assert { :sourceloc "/Users/schaef/git/jar2bpl/jar2bpl_test/regression/false_positives/fp01/FalsePositives01.java",41,9,41,11 } true;
     goto block8;
@@ -206,6 +203,14 @@ var temp$08 : ref;
     assert { :sourceloc "/Users/schaef/git/jar2bpl/jar2bpl_test/regression/false_positives/fp01/FalsePositives01.java",44,6,44,15 } true;
     assert { :sourceloc "/Users/schaef/git/jar2bpl/jar2bpl_test/regression/false_positives/fp01/FalsePositives01.java",44,6,44,15 } temp$917 != $null;
     call temp$1018, $exception := java.lang.String$java.lang.String$toString$124(temp$917);
+    if ($exception != $null) {
+        if ($heap[$exception,$type] <: java.lang.ClassCastException) {
+            assert { :clone } true;
+            goto block9;
+        } else {
+            assert { :clone } true;
+        }
+    }
   block8:
     assert { :sourceloc "/Users/schaef/git/jar2bpl/jar2bpl_test/regression/false_positives/fp01/FalsePositives01.java",44,6,44,15 } true;
     assert { :sourceloc "/Users/schaef/git/jar2bpl/jar2bpl_test/regression/false_positives/fp01/FalsePositives01.java",44,6,44,15 } true;
@@ -220,8 +225,8 @@ var temp$08 : ref;
   block4:
     assert { :sourceloc "/Users/schaef/git/jar2bpl/jar2bpl_test/regression/false_positives/fp01/FalsePositives01.java",32,4,46,4 } true;
     assert { :sourceloc "/Users/schaef/git/jar2bpl/jar2bpl_test/regression/false_positives/fp01/FalsePositives01.java",28,3,51,3 } true;
-    goto block9;
-  block10:
+    goto block10;
+  block9:
     assert { :sourceloc "/Users/schaef/git/jar2bpl/jar2bpl_test/regression/false_positives/fp01/FalsePositives01.java",28,3,51,3 } true;
     assert { :sourceloc "/Users/schaef/git/jar2bpl/jar2bpl_test/regression/false_positives/fp01/FalsePositives01.java",48,3,51,3 } true;
     assert { :sourceloc "/Users/schaef/git/jar2bpl/jar2bpl_test/regression/false_positives/fp01/FalsePositives01.java",48,3,51,3 } $exception != $null;
@@ -229,8 +234,8 @@ var temp$08 : ref;
     cce21 := $exception;
     assert { :sourceloc "/Users/schaef/git/jar2bpl/jar2bpl_test/regression/false_positives/fp01/FalsePositives01.java",48,3,51,3 } true;
     assert { :sourceloc "/Users/schaef/git/jar2bpl/jar2bpl_test/regression/false_positives/fp01/FalsePositives01.java",48,3,51,3 } true;
-    goto block9;
-  block9:
+    goto block10;
+  block10:
     assert { :sourceloc "/Users/schaef/git/jar2bpl/jar2bpl_test/regression/false_positives/fp01/FalsePositives01.java",48,3,51,3 } true;
     assert { :sourceloc "/Users/schaef/git/jar2bpl/jar2bpl_test/regression/false_positives/fp01/FalsePositives01.java",48,3,51,3 } true;
     return;
@@ -239,15 +244,15 @@ var temp$08 : ref;
 
 implementation void$FalsePositives01$FalsePositive01$1892($this:ref) returns ($exception:ref){
     
+var temp$328 : int;    
+var counter24 : int;    
 var temp$227 : int;    
 var temp$025 : int;    
+var hit23 : int;    
 var this22 : ref;    
 var temp$530 : int;    
 var temp$126 : int;    
-var temp$429 : int;    
-var temp$328 : int;    
-var hit23 : int;    
-var counter24 : int;
+var temp$429 : int;
     assume { :sourceloc "/Users/schaef/git/jar2bpl/jar2bpl_test/regression/false_positives/fp01/FalsePositives01.java",-1,-1,-1,-1 } $this != $null;
     assert { :sourceloc "/Users/schaef/git/jar2bpl/jar2bpl_test/regression/false_positives/fp01/FalsePositives01.java",55,2,72,2 } true;
     this22 := $this;
@@ -267,8 +272,6 @@ var counter24 : int;
     if (temp$126 > counter24) {
         assert { :sourceloc "/Users/schaef/git/jar2bpl/jar2bpl_test/regression/false_positives/fp01/FalsePositives01.java",61,7,61,17 } true;
         goto block12;
-    } else {
-        assert { :sourceloc "/Users/schaef/git/jar2bpl/jar2bpl_test/regression/false_positives/fp01/FalsePositives01.java",61,7,61,17 } true;
     }
     assert { :sourceloc "/Users/schaef/git/jar2bpl/jar2bpl_test/regression/false_positives/fp01/FalsePositives01.java",61,7,61,17 } true;
     goto block13;
@@ -288,8 +291,6 @@ var counter24 : int;
     if (counter24 > 10000) {
         assert { :sourceloc "/Users/schaef/git/jar2bpl/jar2bpl_test/regression/false_positives/fp01/FalsePositives01.java",65,8,65,22 } true;
         goto block14;
-    } else {
-        assert { :sourceloc "/Users/schaef/git/jar2bpl/jar2bpl_test/regression/false_positives/fp01/FalsePositives01.java",65,8,65,22 } true;
     }
     assert { :sourceloc "/Users/schaef/git/jar2bpl/jar2bpl_test/regression/false_positives/fp01/FalsePositives01.java",65,8,65,22 } true;
     goto block15;
@@ -306,8 +307,6 @@ var counter24 : int;
     if (hit23 == 0) {
         assert { :sourceloc "/Users/schaef/git/jar2bpl/jar2bpl_test/regression/false_positives/fp01/FalsePositives01.java",70,11,70,13 } true;
         goto block16;
-    } else {
-        assert { :sourceloc "/Users/schaef/git/jar2bpl/jar2bpl_test/regression/false_positives/fp01/FalsePositives01.java",70,11,70,13 } true;
     }
     assert { :sourceloc "/Users/schaef/git/jar2bpl/jar2bpl_test/regression/false_positives/fp01/FalsePositives01.java",70,11,70,13 } true;
     goto block11;
@@ -324,72 +323,68 @@ var counter24 : int;
 
 implementation void$FalsePositives01$FalsePositive02$1893($this:ref, $in_parameter__0:ref) returns ($exception:ref){
     
+var temp$336 : ref;    
+var temp$740 : int;    
+var temp$437 : int;    
+var temp$538 : int;    
+var this31 : ref;    
 var temp$841 : int;    
 var htmlTag32 : ref;    
-var temp$134 : int;    
 var temp$639 : ref;    
-var temp$538 : int;    
-var temp$235 : int;    
 var temp$033 : ref;    
-var temp$437 : int;    
-var temp$740 : int;    
-var temp$336 : ref;    
-var this31 : ref;
+var temp$134 : int;    
+var temp$235 : int;
     assume { :sourceloc "/Users/schaef/git/jar2bpl/jar2bpl_test/regression/false_positives/fp01/FalsePositives01.java",-1,-1,-1,-1 } $this != $null;
     assume $heap[$in_parameter__0,$type] <: java.lang.Object;
     assert { :sourceloc "/Users/schaef/git/jar2bpl/jar2bpl_test/regression/false_positives/fp01/FalsePositives01.java",74,2,87,2 } true;
     this31 := $this;
     assert { :sourceloc "/Users/schaef/git/jar2bpl/jar2bpl_test/regression/false_positives/fp01/FalsePositives01.java",74,30,74,43 } true;
     htmlTag32 := $in_parameter__0;
-    assert { :sourceloc "/Users/schaef/git/jar2bpl/jar2bpl_test/regression/false_positives/fp01/FalsePositives01.java",75,7,75,47 } { :clone } true;
-    assert { :sourceloc "/Users/schaef/git/jar2bpl/jar2bpl_test/regression/false_positives/fp01/FalsePositives01.java",75,7,75,47 } { :clone } htmlTag32 != $null;
+    assert { :sourceloc "/Users/schaef/git/jar2bpl/jar2bpl_test/regression/false_positives/fp01/FalsePositives01.java",75,7,75,47 } true;
+    assert { :sourceloc "/Users/schaef/git/jar2bpl/jar2bpl_test/regression/false_positives/fp01/FalsePositives01.java",75,7,75,47 } htmlTag32 != $null;
     call temp$033, $exception := java.lang.String$java.lang.Object$toString$44(htmlTag32);
-    assert { :sourceloc "/Users/schaef/git/jar2bpl/jar2bpl_test/regression/false_positives/fp01/FalsePositives01.java",75,7,75,47 } { :clone } true;
-    assert { :sourceloc "/Users/schaef/git/jar2bpl/jar2bpl_test/regression/false_positives/fp01/FalsePositives01.java",75,7,75,47 } { :clone } temp$033 != $null;
+    assert { :sourceloc "/Users/schaef/git/jar2bpl/jar2bpl_test/regression/false_positives/fp01/FalsePositives01.java",75,7,75,47 } true;
+    assert { :sourceloc "/Users/schaef/git/jar2bpl/jar2bpl_test/regression/false_positives/fp01/FalsePositives01.java",75,7,75,47 } temp$033 != $null;
     call temp$134 := int$java.lang.String$compareTo$87(temp$033, $StringConst1);
-    assert { :sourceloc "/Users/schaef/git/jar2bpl/jar2bpl_test/regression/false_positives/fp01/FalsePositives01.java",75,7,75,47 } { :clone } true;
+    assert { :sourceloc "/Users/schaef/git/jar2bpl/jar2bpl_test/regression/false_positives/fp01/FalsePositives01.java",75,7,75,47 } true;
     if (temp$134 == 0) {
-        assert { :sourceloc "/Users/schaef/git/jar2bpl/jar2bpl_test/regression/false_positives/fp01/FalsePositives01.java",75,7,75,47 } { :clone } true;
+        assert { :sourceloc "/Users/schaef/git/jar2bpl/jar2bpl_test/regression/false_positives/fp01/FalsePositives01.java",75,7,75,47 } true;
         goto block17;
-    } else {
-        assert { :sourceloc "/Users/schaef/git/jar2bpl/jar2bpl_test/regression/false_positives/fp01/FalsePositives01.java",75,7,75,47 } { :clone } true;
     }
-    assert { :sourceloc "/Users/schaef/git/jar2bpl/jar2bpl_test/regression/false_positives/fp01/FalsePositives01.java",75,7,75,47 } { :clone } true;
+    assert { :sourceloc "/Users/schaef/git/jar2bpl/jar2bpl_test/regression/false_positives/fp01/FalsePositives01.java",75,7,75,47 } true;
     goto block18;
   block17:
-    assert { :sourceloc "/Users/schaef/git/jar2bpl/jar2bpl_test/regression/false_positives/fp01/FalsePositives01.java",75,7,75,47 } { :clone } true;
+    assert { :sourceloc "/Users/schaef/git/jar2bpl/jar2bpl_test/regression/false_positives/fp01/FalsePositives01.java",75,7,75,47 } true;
     assert { :sourceloc "/Users/schaef/git/jar2bpl/jar2bpl_test/regression/false_positives/fp01/FalsePositives01.java",77,4,77,14 } true;
     temp$235 := 1;
     assert { :sourceloc "/Users/schaef/git/jar2bpl/jar2bpl_test/regression/false_positives/fp01/FalsePositives01.java",77,4,77,14 } true;
     $heap := $heap[this31,int$FalsePositives01$countSource0 := temp$235];
-    assert { :sourceloc "/Users/schaef/git/jar2bpl/jar2bpl_test/regression/false_positives/fp01/FalsePositives01.java",75,3,86,3 } { :clone } true;
+    assert { :sourceloc "/Users/schaef/git/jar2bpl/jar2bpl_test/regression/false_positives/fp01/FalsePositives01.java",75,3,86,3 } true;
     goto block19;
   block18:
-    assert { :sourceloc "/Users/schaef/git/jar2bpl/jar2bpl_test/regression/false_positives/fp01/FalsePositives01.java",75,3,86,3 } { :clone } true;
-    assert { :sourceloc "/Users/schaef/git/jar2bpl/jar2bpl_test/regression/false_positives/fp01/FalsePositives01.java",79,12,79,49 } { :clone } true;
+    assert { :sourceloc "/Users/schaef/git/jar2bpl/jar2bpl_test/regression/false_positives/fp01/FalsePositives01.java",75,3,86,3 } true;
+    assert { :sourceloc "/Users/schaef/git/jar2bpl/jar2bpl_test/regression/false_positives/fp01/FalsePositives01.java",79,12,79,49 } true;
     call temp$336, $exception := java.lang.String$java.lang.Object$toString$44(htmlTag32);
-    assert { :sourceloc "/Users/schaef/git/jar2bpl/jar2bpl_test/regression/false_positives/fp01/FalsePositives01.java",79,12,79,49 } { :clone } true;
-    assert { :sourceloc "/Users/schaef/git/jar2bpl/jar2bpl_test/regression/false_positives/fp01/FalsePositives01.java",79,12,79,49 } { :clone } temp$336 != $null;
+    assert { :sourceloc "/Users/schaef/git/jar2bpl/jar2bpl_test/regression/false_positives/fp01/FalsePositives01.java",79,12,79,49 } true;
+    assert { :sourceloc "/Users/schaef/git/jar2bpl/jar2bpl_test/regression/false_positives/fp01/FalsePositives01.java",79,12,79,49 } temp$336 != $null;
     call temp$437 := int$java.lang.String$compareTo$87(temp$336, $StringConst2);
-    assert { :sourceloc "/Users/schaef/git/jar2bpl/jar2bpl_test/regression/false_positives/fp01/FalsePositives01.java",79,12,79,49 } { :clone } true;
+    assert { :sourceloc "/Users/schaef/git/jar2bpl/jar2bpl_test/regression/false_positives/fp01/FalsePositives01.java",79,12,79,49 } true;
     if (temp$437 == 0) {
-        assert { :sourceloc "/Users/schaef/git/jar2bpl/jar2bpl_test/regression/false_positives/fp01/FalsePositives01.java",79,12,79,49 } { :clone } true;
+        assert { :sourceloc "/Users/schaef/git/jar2bpl/jar2bpl_test/regression/false_positives/fp01/FalsePositives01.java",79,12,79,49 } true;
         goto block20;
-    } else {
-        assert { :sourceloc "/Users/schaef/git/jar2bpl/jar2bpl_test/regression/false_positives/fp01/FalsePositives01.java",79,12,79,49 } { :clone } true;
     }
-    assert { :sourceloc "/Users/schaef/git/jar2bpl/jar2bpl_test/regression/false_positives/fp01/FalsePositives01.java",79,12,79,49 } { :clone } true;
+    assert { :sourceloc "/Users/schaef/git/jar2bpl/jar2bpl_test/regression/false_positives/fp01/FalsePositives01.java",79,12,79,49 } true;
     goto block21;
   block20:
-    assert { :sourceloc "/Users/schaef/git/jar2bpl/jar2bpl_test/regression/false_positives/fp01/FalsePositives01.java",79,12,79,49 } { :clone } true;
+    assert { :sourceloc "/Users/schaef/git/jar2bpl/jar2bpl_test/regression/false_positives/fp01/FalsePositives01.java",79,12,79,49 } true;
     assert { :sourceloc "/Users/schaef/git/jar2bpl/jar2bpl_test/regression/false_positives/fp01/FalsePositives01.java",81,4,81,14 } true;
     temp$538 := 2;
     assert { :sourceloc "/Users/schaef/git/jar2bpl/jar2bpl_test/regression/false_positives/fp01/FalsePositives01.java",81,4,81,14 } true;
     $heap := $heap[this31,int$FalsePositives01$countSource0 := temp$538];
-    assert { :sourceloc "/Users/schaef/git/jar2bpl/jar2bpl_test/regression/false_positives/fp01/FalsePositives01.java",79,8,86,3 } { :clone } true;
+    assert { :sourceloc "/Users/schaef/git/jar2bpl/jar2bpl_test/regression/false_positives/fp01/FalsePositives01.java",79,8,86,3 } true;
     goto block22;
   block21:
-    assert { :sourceloc "/Users/schaef/git/jar2bpl/jar2bpl_test/regression/false_positives/fp01/FalsePositives01.java",79,8,86,3 } { :clone } true;
+    assert { :sourceloc "/Users/schaef/git/jar2bpl/jar2bpl_test/regression/false_positives/fp01/FalsePositives01.java",79,8,86,3 } true;
     assert { :sourceloc "/Users/schaef/git/jar2bpl/jar2bpl_test/regression/false_positives/fp01/FalsePositives01.java",83,12,83,49 } true;
     call temp$639, $exception := java.lang.String$java.lang.Object$toString$44(htmlTag32);
     assert { :sourceloc "/Users/schaef/git/jar2bpl/jar2bpl_test/regression/false_positives/fp01/FalsePositives01.java",83,12,83,49 } true;
@@ -399,8 +394,6 @@ var this31 : ref;
     if (temp$740 == 0) {
         assert { :sourceloc "/Users/schaef/git/jar2bpl/jar2bpl_test/regression/false_positives/fp01/FalsePositives01.java",83,12,83,49 } true;
         goto block23;
-    } else {
-        assert { :sourceloc "/Users/schaef/git/jar2bpl/jar2bpl_test/regression/false_positives/fp01/FalsePositives01.java",83,12,83,49 } true;
     }
     assert { :sourceloc "/Users/schaef/git/jar2bpl/jar2bpl_test/regression/false_positives/fp01/FalsePositives01.java",83,12,83,49 } true;
     goto block24;
@@ -424,24 +417,24 @@ var this31 : ref;
 implementation void$FalsePositives01$FalsePositive03$1894($this:ref, $in_parameter__0:ref, $in_parameter__1:ref, $in_parameter__2:int) returns ($exception:ref){
     
 var temp$453 : int;    
-var hitUp48 : int;    
-var temp$150 : int;    
-var temp$857 : int;    
-var source43 : ref;    
-var temp$352 : int;    
-var temp$251 : int;    
 var temp$756 : int;    
+var this42 : ref;    
+var searchString44 : ref;    
+var temp$049 : int;    
+var temp$251 : int;    
 var flaghitup47 : int;    
 var temphitpoint46 : int;    
-var temp$655 : int;    
-var this42 : ref;    
-var interncaret45 : int;    
-var temp$049 : int;    
 var temp$554 : int;    
-var searchString44 : ref;
+var temp$655 : int;    
+var source43 : ref;    
+var temp$150 : int;    
+var interncaret45 : int;    
+var hitUp48 : int;    
+var temp$857 : int;    
+var temp$352 : int;
     assume { :sourceloc "/Users/schaef/git/jar2bpl/jar2bpl_test/regression/false_positives/fp01/FalsePositives01.java",-1,-1,-1,-1 } $this != $null;
-    assume $heap[$in_parameter__0,$type] <: java.lang.String;
     assume $heap[$in_parameter__1,$type] <: java.lang.String;
+    assume $heap[$in_parameter__0,$type] <: java.lang.String;
     assert { :sourceloc "/Users/schaef/git/jar2bpl/jar2bpl_test/regression/false_positives/fp01/FalsePositives01.java",90,2,111,2 } true;
     this42 := $this;
     assert { :sourceloc "/Users/schaef/git/jar2bpl/jar2bpl_test/regression/false_positives/fp01/FalsePositives01.java",90,30,90,42 } true;
@@ -471,8 +464,6 @@ var searchString44 : ref;
     if (temphitpoint46 > 0) {
         assert { :sourceloc "/Users/schaef/git/jar2bpl/jar2bpl_test/regression/false_positives/fp01/FalsePositives01.java",98,7,98,22 } true;
         goto block26;
-    } else {
-        assert { :sourceloc "/Users/schaef/git/jar2bpl/jar2bpl_test/regression/false_positives/fp01/FalsePositives01.java",98,7,98,22 } true;
     }
     assert { :sourceloc "/Users/schaef/git/jar2bpl/jar2bpl_test/regression/false_positives/fp01/FalsePositives01.java",98,7,98,22 } true;
     goto block27;
@@ -484,8 +475,6 @@ var searchString44 : ref;
     if (temphitpoint46 < temp$251) {
         assert { :sourceloc "/Users/schaef/git/jar2bpl/jar2bpl_test/regression/false_positives/fp01/FalsePositives01.java",98,42,98,52 } true;
         goto block28;
-    } else {
-        assert { :sourceloc "/Users/schaef/git/jar2bpl/jar2bpl_test/regression/false_positives/fp01/FalsePositives01.java",98,42,98,52 } true;
     }
     assert { :sourceloc "/Users/schaef/git/jar2bpl/jar2bpl_test/regression/false_positives/fp01/FalsePositives01.java",98,42,98,52 } true;
     goto block27;
@@ -518,8 +507,6 @@ var searchString44 : ref;
     if (flaghitup47 == 0) {
         assert { :sourceloc "/Users/schaef/git/jar2bpl/jar2bpl_test/regression/false_positives/fp01/FalsePositives01.java",104,11,104,19 } true;
         goto block29;
-    } else {
-        assert { :sourceloc "/Users/schaef/git/jar2bpl/jar2bpl_test/regression/false_positives/fp01/FalsePositives01.java",104,11,104,19 } true;
     }
     assert { :sourceloc "/Users/schaef/git/jar2bpl/jar2bpl_test/regression/false_positives/fp01/FalsePositives01.java",104,11,104,19 } true;
     goto block25;
@@ -529,8 +516,6 @@ var searchString44 : ref;
     if (hitUp48 == 0) {
         assert { :sourceloc "/Users/schaef/git/jar2bpl/jar2bpl_test/regression/false_positives/fp01/FalsePositives01.java",105,6,105,15 } true;
         goto block30;
-    } else {
-        assert { :sourceloc "/Users/schaef/git/jar2bpl/jar2bpl_test/regression/false_positives/fp01/FalsePositives01.java",105,6,105,15 } true;
     }
     assert { :sourceloc "/Users/schaef/git/jar2bpl/jar2bpl_test/regression/false_positives/fp01/FalsePositives01.java",105,6,105,15 } true;
     goto block31;
